backends/lean/Aeneas/Std/Alloc.lean
@@ -20,12 +20,14 @@ def alloc.boxed.Box.deref {T : Type} (x : T) : T := x
 def alloc.boxed.Box.deref_mut {T : Type} (x : T) : (T × (T → T)) := (x, λ x => x)
 
 /-- Trait instance -/
+@[rust_trait_impl "core::ops::deref::Deref<Box<@T>, @T>"]
 def core.ops.deref.DerefBoxInst (T : Type) :
   core.ops.deref.Deref T T := {
   deref x := ok (alloc.boxed.Box.deref x)
 }
 
 /-- Trait instance -/
+@[rust_trait_impl "core::ops::deref::DerefMut<Box<@T>, @T>"]
 def core.ops.deref.DerefMutBoxInst (T : Type) :
   core.ops.deref.DerefMut T T := {
   derefInst := DerefBoxInst T
