backends/lean/Aeneas/Std/Array/ArraySlice.lean
@@ -92,18 +92,18 @@ def core.array.Array.index_mut
   let (s, back) ← inst.index_mut a.to_slice i
   ok (s, fun o => Array.from_slice a (back o))
 
-/- Trait implementation: [core::array::[T; N]] -/
-def core.ops.index.IndexArrayInst {T I Output : Type} {N : Usize}
+@[rust_trait_impl "core::ops::index::Index<[@T; @N], @I, @O>"]
+def core.ops.index.IndexArray {T I Output : Type} {N : Usize}
   (inst : core.ops.index.Index (Slice T) I Output) :
   core.ops.index.Index (Array T N) I Output := {
   index := core.array.Array.index inst
 }
 
-/- Trait implementation: [core::array::[T; N]] -/
-def core.ops.index.IndexMutArrayInst {T I Output : Type} {N : Usize}
+@[rust_trait_impl "core::ops::index::IndexMut<[@T; @N], @I, @O>"]
+def core.ops.index.IndexMutArray {T I Output : Type} {N : Usize}
   (inst : core.ops.index.IndexMut (Slice T) I Output) :
   core.ops.index.IndexMut (Array T N) I Output := {
-  indexInst := core.ops.index.IndexArrayInst inst.indexInst
+  indexInst := core.ops.index.IndexArray inst.indexInst
   index_mut := core.array.Array.index_mut inst
 }
 
